\documentclass[letterpaper,notitlepage,11pt]{article}
\usepackage{amsmath}
\usepackage{amssymb}
\usepackage{wasysym}
\begin{document}
\begin{equation}
\frac{a}{b}
\end{equation}
\begin{equation}
\frac{\frac{a}{b}}{\frac{c+d}{d+e}}
\end{equation}
\begin{equation}
\frac12=\frac24=\frac{a}b=\frac{a}{b}
\end{equation}
$\frac{a}{b}$

$\frac{\frac{a}{b}}{\frac{c+d}{d+e}}$

$\frac12=\frac24=\frac{a}b=\frac{a}{b}$

\begin{equation}
F = G_N \frac{m_1 m_2}{r^2}
\end{equation}

\begin{equation}
n_{\pm}(E,T)=\frac1{e^{\frac{E}{k_BT}}\pm1} =\frac1{e^{{\hbar\omega}/{k_BT}}\pm1}
\end{equation}

\begin{equation}
F_{\mu \nu} = [D_\mu, D_\nu] = \partial_\mu A_\nu-\partial_\nu A_\mu = \partial_{[\mu} A_{\nu]}
\end{equation}

$\frac{1}{2}$

\(\tfrac12\)

\[ \frac{1}{2} \]

\[ \frac12a+b\]

\[ \tfrac12a+b\]

\newpage

\begin{equation}
\frac{df}{dt}
\end{equation}

\begin{equation}
\frac{\partial f}{\partial t}
\end{equation}

\begin{equation}
\int f(x) dx, \sum x_n, \prod \omega_k
\end{equation}

\begin{equation}
\int_0^1 f(x)dx, \sum_{n=0}^7 x_n, \prod_1^{10} \omega_k
\end{equation}

\begin{equation}
\int^1_0 f(x)dx, \sum^7_{n=0} x_n, \prod^{10}_1 \omega_k
\end{equation}

$\int_0^1 f(x)dx, \sum_{n=0}^7 x_n, \prod_1^{10} \omega_k$

\[ e^x=\sum^\infty_{n=0} \frac1{n!}x^n \]

``Taylor expansion $e^x=\sum_{n=0}^\infty \frac1{n!}x^n$.''

\begin{equation}
\int^1_0 \frac{df}{dx}dx = f(1) - f(0)
\end{equation}

\begin{equation}
e^{\zeta(s)} = \prod^\infty_{n=1} e^{1/n^s}
\end{equation}

\newpage

\begin{equation}
(\frac12 a+\frac{x+y}{z+d})
\end{equation}

\begin{equation}
\left(\frac12 a+\frac{x+y}{z+d}\right)
\end{equation}

$\{ \}$

\begin{equation}
\left\langle\frac12 a+\frac{x+y}{z+d}\right]
\end{equation}

\begin{equation}
\left\langle\frac{ab}{cd} \frac{cd}{ef}\right\rangle
\end{equation}

\begin{equation}
\left\langle\frac12 a+\frac{x+y}{z+d}\right.
\end{equation}

\begin{equation}
\left. \frac{df}{dt} \right|_{t=0}
\end{equation}

\end{document}